src/graph_theory/path.lean
@@ -39,30 +39,30 @@ namespace Graph
         @[simp] lemma size_concat {p : path G x y} {p' : path G y z} : (concat p p').size = p.size + p'.size
             := llist.concat_size 
 
-        def edges_aux : Π (l : llist V) (h : llist.is_path G.adj l), list (edge G)
+        def edges_aux : Π (l : llist V) (h : llist.is_path G.adj l), list (edges G)
             | (llist.pt v)   _ := []
             | (llist.cons v l) h := ⟨h.1⟩ :: edges_aux l h.2
 
-        def edges (p : path G x y) : list (edge G)
+        def all_edges (p : path G x y) : list (edges G)
             := edges_aux p.l p.adj
 
-        lemma mem_edges_aux' {l h} {e : edge G} : e ∈ @edges_aux V G l h -> e.x ∈ l.init ∧ e.y ∈ l.tail
+        lemma mem_edges_aux' {l h} {e : edges G} : e ∈ @edges_aux V G l h -> e.x ∈ l.init ∧ e.y ∈ l.tail
             := by { induction l with v v l hr; intros he; cases he with he he,
                 { subst he, split; left; refl },
                 { cases hr he, split; right; assumption } }
 
-        lemma mem_edges_aux {l h} {e : edge G} : e ∈ @edges_aux V G l h -> e.x ∈ l ∧ e.y ∈ l
+        lemma mem_edges_aux {l h} {e : edges G} : e ∈ @edges_aux V G l h -> e.x ∈ l ∧ e.y ∈ l
             := by { intro h1, cases mem_edges_aux' h1 with h2 h3, split, 
                 { exact llist.mem_init_last.mpr (or.inl h2) },
                 { exact llist.mem_head_tail.mpr (or.inr h3) } }
 
-        lemma mem_edges {p : path G x y} {e : edge G} : e ∈ p.edges -> e.x ∈ p ∧ e.y ∈ p
+        lemma mem_edges {p : path G x y} {e : edges G} : e ∈ p.all_edges -> e.x ∈ p ∧ e.y ∈ p
             := mem_edges_aux
 
-        lemma edges_simple {l} (h) (hs : llist.nodup l) : list.pairwise (edge.nsame G) (@edges_aux V G l h)
+        lemma edges_simple {l} (h) (hs : llist.nodup l) : list.pairwise edges.nsame (@edges_aux V G l h)
             := by { induction l with v v l hr, { exact list.pairwise.nil },
                 { apply list.pairwise.cons, 
-                { intros e he, rw [edge.nsame, edge.same], push_neg, have h5 := mem_edges_aux he,
+                { intros e he, rw [edges.nsame, edges.same], push_neg, have h5 := mem_edges_aux he,
                     split; intro h6; subst h6, exact hs.1 h5.1, exact hs.1 h5.2 },
                 { exact hr h.2 hs.2 } } }
 
@@ -98,7 +98,7 @@ namespace Graph
         def rev (p : spath G x y) : spath G y x
             := ⟨p.to_path.rev, llist.nodup_rev.mpr p.simple⟩
 
-        lemma edges_simple {p : spath G x y} : list.pairwise (edge.nsame G) p.to_path.edges
+        lemma edges_simple {p : spath G x y} : list.pairwise edges.nsame p.to_path.all_edges
             := path.edges_simple _ p.simple
     end spath
 end Graph
